Code/Database.fst
@@ -1,6 +1,5 @@
 module Database
 
-open SamlProtocol
 open Crypto
 open CertStore
 open TypeFunc
@@ -8,14 +7,17 @@ open TypeFunc
 (*Identity provider functionality*)
 val whitelist: idp:prin -> unit
 val blacklist: idp:prin -> unit
-val addidp: idp:prin -> unit
+val addidp: idp:prin -> bool
 val whitelisted: idp:prin -> bool
 
 (*User functionality*)
-val adduser: user:string -> password:string -> unit
+val createuser: user:prin -> userid:string -> password:string -> bool
+val usercreation: user:prin -> generatedPassword:string -> bool
+val changeuserid: user:string -> newuser:string -> password:string -> bool
+val changeuserpassword: user:string -> password:string -> newpassword:string -> bool
 
-val addnfactor: user:string -> nfactor:Authentication -> unit
-val removenfactor: user:string -> nfactor:Authentication -> unit
+val addnfactor: user:string -> password:string -> nfactor:Authentication -> bool
+val removenfactor: user:string -> password:string -> nfactor:Authentication -> bool
 
 val getnfactor: user:string -> Authentication
 val checknfactor: user:string -> Authentication -> bool
@@ -24,6 +26,6 @@ val resetnfact: user:string -> unit
 
 val checklogin: user:string -> password:string -> bool
 
-val revokeidp: user:string -> idp:prin -> unit
+val revokeidp: user:string -> password:string -> idp:string -> bool
 
 val revokedidp: user:string -> idp:prin -> bool
